transversal finite wip

Matroid/Transversal.lean
@@ -1,20 +1,36 @@
 import Matroid.Simple
-open Set
+import Mathlib.combinatorics.hall.basic
 namespace Matroid
+open Finset
 
-structure family_over (ι : Type _) (S : Set α) where
-  (index : ι → Set α)
-  (mem_subset : ∀ ι, index ι ⊆ S)
 
-def Function.transversal {S : Set α} {ι : Type _} (T : Set α) (T_map : α → ι)
-    (f : family_over ι S): Prop :=
-  (∀ t ∈ T, t ∈ f.index (T_map t)) ∧ T.InjOn T_map
 
-def Set.transverses (T : Set α) {S : Set α} {ι : Type _} (f : family_over ι S) : Prop :=
-  ∃ (T_map : α → ι), Function.transversal T T_map f
+def transverses (T : Finset α) {ι : Type _} (f : ι → Finset α): Prop :=
+  ∃ (m : α → ι), Set.InjOn m T.toSet ∧ (∀ a, a ∈ T → a ∈ f (m a))
+
+theorem transverses_iff_hall (T : Finset α) (f : ι → Finset α):
+    transverses T f ↔ ∀ S, S ⊆ T → S.card ≥ (S.biUnion f) := sorry
+
+def matroid_of_transversals_finite {ι a : Type _} [DecidableEq α] [Inhabited ι] [Fintype ι]
+    (f : ι → Finset α) : Matroid α :=
+  matroid_of_indep_finset (Finset.univ.biUnion f)
+  (fun S ↦ transverses S f)
+  (⟨(fun a ↦ default), ⟨fun a a_mem ↦ absurd a_mem (not_mem_empty a),
+    fun a a_mem ↦ absurd a_mem (not_mem_empty a)⟩⟩)
+  (by
+    rintro I J ⟨J_map, J_map_inj, h_J_map⟩ I_sub
+    refine' ⟨J_map, J_map_inj.mono I_sub, fun a a_T ↦ h_J_map a (I_sub a_T)⟩
+  )
+  (by
+    rintro I J ⟨I_map, I_map_inj, h_I_map⟩ ⟨J_map, J_map_inj, h_J_map⟩ I_lt_J
+    sorry
+  )
+
+   sorry
+
 
 /-
-def Function.total_transversal {S : Set α} {ι : Type _} (T : Set α) (T_map : α → ι) 
+def Function.total_transversal {S : Set α} {ι : Type _} (T : Set α) (T_map : α → ι)
     (f : family_over ι S) : Prop :=
   Function.transversal T T_map f ∧ T.BijOn T_map univ
 
@@ -22,11 +38,14 @@ def Set.total_transverses (T : Set α) {S : Set α} {ι : Type _} (f : family_ov
   ∃ (T_map : α → ι), Function.total_transversal T T_map f
 -/
 
+def Function.pairs (f : α → β) := {x : Prod α β | f x.1 = x.2}
+
+
 
 
 lemma transversal_not_maximal_of_open_pair [DecidableEq α]{T : Set α} {f : family_over ι S} {T_map : α → ι}
     (T_map_trans : Function.transversal T T_map f) {s : α} {i : ι} (s_i : s ∈ f.index i)
-    (s_nT : s ∉ T) (i_nT : i ∉ T_map '' T) : 
+    (s_nT : s ∉ T) (i_nT : i ∉ T_map '' T) :
     T ∉ maximals (fun x x_1 ↦ x ⊆ x_1) {I | Set.transverses I f} := by
   intro T_max
   set T_map' := Function.update T_map s i
@@ -47,33 +66,9 @@ lemma transversal_not_maximal_of_open_pair [DecidableEq α]{T : Set α} {f : fam
       exfalso
       exact i_nT ⟨b, b_mem_T, abeq (ne_of_mem_of_not_mem b_mem_T s_nT)⟩
   · obtain ((b_eq_s : b = s) | b_mem_T) := b_mem
-    · rw [b_eq_s, Function.update_same, Function.update_apply, ite_eq_left_iff] at abeq 
+    · rw [b_eq_s, Function.update_same, Function.update_apply, ite_eq_left_iff] at abeq
       exfalso
       exact i_nT ⟨a, a_mem_T, abeq (ne_of_mem_of_not_mem a_mem_T s_nT)⟩
-    · rw [Function.update_noteq (ne_of_mem_of_not_mem a_mem_T s_nT), 
+    · rw [Function.update_noteq (ne_of_mem_of_not_mem a_mem_T s_nT),
     Function.update_noteq (ne_of_mem_of_not_mem b_mem_T s_nT), ] at abeq
       exact T_map_trans.2 a_mem_T b_mem_T abeq
-
-
-
-def matroid_of_transversals {S : Set α} {ι : Type _} [Inhabited ι] (f : family_over ι S) : Matroid α :=
-  matroid_of_indep S (fun I ↦ Set.transverses I f)
-  (⟨(fun a ↦ default), ⟨fun t t_mem ↦ absurd t_mem (not_mem_empty t), fun a a_mem ↦ absurd a_mem (not_mem_empty a)⟩⟩) 
-  (fun I J ⟨J_map, h_J_map⟩ I_sub ↦ ⟨J_map, ⟨fun t t_mem ↦ h_J_map.1 t (I_sub t_mem), Set.InjOn.mono I_sub h_J_map.2⟩⟩)
-  (by
-    rintro I J ⟨I_map, h_I_map⟩ I_not_max J_max
-    have not_J_sub_I : ¬ J ⊆ I
-    · intro J_sub_I
-      apply I_not_max ⟨⟨I_map, h_I_map⟩, _⟩
-      intro B B_ind I_sub_B
-      exact subset_trans (J_max.2 B_ind (subset_trans J_sub_I I_sub_B)) J_sub_I
-    obtain ⟨j, j_J, j_nI⟩ := not_subset_iff_exists_mem_not_mem.1 not_J_sub_I
-    refine' ⟨j, ⟨j_J, j_nI⟩, _⟩
-    dsimp
-    
-
-
-
-  ) 
-  sorry sorry
-
